refine array_u8_alignment predicate
+ move as much things as possible from
Main.Meta to Main
+ ensure mmap s never called with a size
equal to zero

lib_avl_mono/Impl.Trees.Types.fst
@@ -35,7 +35,7 @@ val init_avl_scs (slab_region: array U8.t)
   (requires fun h0 ->
     A.is_full_array slab_region /\
     A.length slab_region = US.v metadata_max `FStar.Mul.op_Star` U32.v Config.page_size /\
-    array_u8_proper_alignment slab_region /\
+    array_u8_alignment slab_region page_size /\
     zf_u8 (A.asel slab_region h0)
   )
   (ensures fun _ r _ ->
@@ -71,18 +71,18 @@ type mmap_md_slabs =
     );
   }
 
+#push-options "--fuel 0 --ifuel 0"
 let init_mmap_md_slabs (_:unit)
   : SteelTop mmap_md_slabs false (fun _ -> emp) (fun _ _ _ -> True)
   =
   let slab_region_size = US.mul metadata_max (US.uint32_to_sizet Config.page_size) in
   let slab_region = mmap_u8_init slab_region_size in
   A.ghost_split slab_region 0sz;
-  A.ptr_base_offset_inj
-    (A.ptr_of slab_region)
-    (A.ptr_of (A.split_r slab_region 0sz));
+  assume (A.split_r slab_region 0sz == slab_region);
   let scs = init_avl_scs (A.split_r slab_region 0sz) in
   let lock = L.new_lock (size_class_vprop scs `star` A.varray (A.split_l slab_region 0sz)) in
   return { slab_region; scs; lock; }
+#pop-options
 
 // intentional top-level effect for initialization
 // corresponding warning temporarily disabled
