src/Main.Meta.fsti
@@ -24,11 +24,8 @@ open Mman
 open Config
 open Utils2
 open NullOrVarray
-open Main
 open ROArray
-
-/// An attribute, that will indicate that the annotated functions should be unfolded at compile-time
-irreducible let reduce_attr : unit = ()
+open Main
 
 /// The total number of size classes in the allocator, across all arenas.
 /// Used as an abbreviation for specification purposes
@@ -79,7 +76,7 @@ val slab_malloc
       = h1 (null_or_varray r) in
     not (is_null r) ==> (
       A.length r >= U32.v bytes /\
-      array_u8_proper_alignment r /\
+      array_u8_alignment r 16ul /\
       Seq.length s >= 2 /\
       (enable_slab_canaries_malloc ==>
         Seq.index s (A.length r - 2) == slab_canaries_magic1 /\
@@ -88,25 +85,25 @@ val slab_malloc
     )
   )
 
-[@@ T.postprocess_with norm_full]
-val slab_aligned_alloc (arena_id:US.t{US.v arena_id < US.v nb_arenas}) (alignment:U32.t) (bytes:U32.t)
-  : Steel (array U8.t)
-  emp
-  (fun r -> null_or_varray r)
-  (requires fun _ -> True)
-  (ensures fun _ r h1 ->
-    let s : t_of (null_or_varray r)
-      = h1 (null_or_varray r) in
-    not (is_null r) ==> (
-      A.length r >= U32.v bytes /\
-      array_u8_proper_alignment r /\
-      Seq.length s >= 2 /\
-      (enable_slab_canaries_malloc ==>
-        Seq.index s (A.length r - 2) == slab_canaries_magic1 /\
-        Seq.index s (A.length r - 1) == slab_canaries_magic2
-      )
-    )
-  )
+//[@@ T.postprocess_with norm_full]
+//val slab_aligned_alloc (arena_id:US.t{US.v arena_id < US.v nb_arenas}) (alignment:U32.t) (bytes:U32.t)
+//  : Steel (array U8.t)
+//  emp
+//  (fun r -> null_or_varray r)
+//  (requires fun _ -> True)
+//  (ensures fun _ r h1 ->
+//    let s : t_of (null_or_varray r)
+//      = h1 (null_or_varray r) in
+//    not (is_null r) ==> (
+//      A.length r >= U32.v bytes /\
+//      array_u8_proper_alignment r /\
+//      Seq.length s >= 2 /\
+//      (enable_slab_canaries_malloc ==>
+//        Seq.index s (A.length r - 2) == slab_canaries_magic1 /\
+//        Seq.index s (A.length r - 1) == slab_canaries_magic2
+//      )
+//    )
+//  )
 
 val within_size_classes_pred (ptr:A.array U8.t) : prop
 
