src/Utils2.fsti
@@ -24,25 +24,28 @@ unfold let same_base_array (#a: Type) (arr1 arr2: array a)
 
 unfold let slab_metadata = r:array U64.t{A.length r = 4}
 
-// abstract property that the underlying pointer is 16-bytes aligned
+// abstract property that the underlying pointer v-bytes aligned
 //assume
-val array_u8_proper_alignment (arr: array U8.t): prop
+val array_u8_alignment (arr: array U8.t) (v: U32.t{U32.v v > 0}): prop
 
 // no model for the memory considered as the "root" array in a tree-like representation
 // thus, this *axiom* is required
-// to convey that if arr (of type uint8_t*) is 16-bytes aligned,
-// then so is, forall k, arr[16*k]
+// to convey that if arr (of type uint8_t*) is v1-bytes aligned,
+// that v1 is a multiple of v2,
+// then forall k,
+// then arr[k * v2] is v2-bytes aligned
 //assume
-val array_u8_proper_alignment_lemma
-  (arr1: array U8.t)
-  (arr2: array U8.t)
+val array_u8_alignment_lemma
+  (arr1 arr2: array U8.t)
+  (v1 v2: (v:U32.t{U32.v v > 0}))
   : Lemma
   (requires
     same_base_array arr1 arr2 /\
-    array_u8_proper_alignment arr1 /\
-    (A.offset (A.ptr_of arr2) - A.offset (A.ptr_of arr1)) % 16 == 0)
+    array_u8_alignment arr1 v1 /\
+    (U32.v v1) % (U32.v v2) == 0 /\
+    (A.offset (A.ptr_of arr2) - A.offset (A.ptr_of arr1)) % (U32.v v2) == 0)
   (ensures
-    array_u8_proper_alignment arr2)
+    array_u8_alignment arr2 v2)
 
 let nb_slots (size_class: sc)
   : Pure U32.t
